src/lowparse/pulse/LowParse.PulseParse.VLData.fst
@@ -322,3 +322,58 @@ fn validate_bounded_vldata_strong
 {
   validate_bounded_vldata_strong' min max (log256' max) s v lr () input poffset
 }
+
+(* zero_copy_parse_bounded_vldata_payload': access the payload of bounded vldata *)
+
+#push-options "--z3rlimit 64"
+
+inline_for_extraction
+fn zero_copy_parse_bounded_vldata_payload'
+  (#tl #t: Type0) (#vmatch: tl -> t -> slprop)
+  (#k: Ghost.erased parser_kind) (#p: parser k t)
+  (min: nat)
+  (max: nat { min <= max /\ max > 0 /\ max < 4294967296 })
+  (l: nat { l >= log256' max /\ l <= 4 })
+  (w: PPB.zero_copy_parse vmatch p)
+  (lr: PPB.leaf_reader (parse_bounded_integer l))
+  (u: squash FStar.SizeT.fits_u64)
+: PPB.zero_copy_parse vmatch (parse_bounded_vldata' min max l p)
+= (input: _)
+  (#pm: _)
+  (#v: _)
+{
+  PPB.pts_to_parsed_elim input;
+  with bytes . assert (S.pts_to input #pm bytes);
+  S.pts_to_len input;
+  SZ.fits_u64_implies_fits_32 ();
+  let l_sz = SZ.uint32_to_sizet (U32.uint_to_t l);
+  parser_kind_prop_equiv (parse_bounded_integer_kind l) (parse_bounded_integer l);
+  Seq.lemma_eq_elim (Seq.slice bytes 0 (Seq.length bytes)) bytes;
+  parse_bounded_vldata_elim' min max l p bytes v (Seq.length bytes);
+  let len = PPB.read_parsed_from_validator_success lr input 0sz l_sz;
+  let input_prefix, input_payload = split_trade input l_sz;
+  with wb_prefix . assert (S.pts_to input_prefix #pm wb_prefix);
+  with wb_payload . assert (S.pts_to input_payload #pm wb_payload);
+  Trade.elim_hyp_l (S.pts_to input_prefix #pm wb_prefix) (S.pts_to input_payload #pm wb_payload) (S.pts_to input #pm bytes);
+  Trade.trans (S.pts_to input_payload #pm wb_payload) (S.pts_to input #pm bytes) (PPB.pts_to_parsed (parse_bounded_vldata' min max l p) input #pm v);
+  Seq.lemma_eq_elim wb_payload (Seq.slice bytes (SZ.v l_sz) (SZ.v l_sz + U32.v len));
+  PPB.pts_to_parsed_intro p input_payload v;
+  Trade.trans (PPB.pts_to_parsed p input_payload #(pm /. 2.0R) v) (S.pts_to input_payload #pm wb_payload) (PPB.pts_to_parsed (parse_bounded_vldata' min max l p) input #pm v);
+  let res = w input_payload;
+  Trade.trans (vmatch res v) (PPB.pts_to_parsed p input_payload #(pm /. 2.0R) v) (PPB.pts_to_parsed (parse_bounded_vldata' min max l p) input #pm v);
+  res
+}
+
+#pop-options
+
+inline_for_extraction
+let zero_copy_parse_bounded_vldata_payload
+  (#tl #t: Type0) (#vmatch: tl -> t -> slprop)
+  (#k: Ghost.erased parser_kind) (#p: parser k t)
+  (min: nat)
+  (max: nat { min <= max /\ max > 0 /\ max < 4294967296 })
+  (w: PPB.zero_copy_parse vmatch p)
+  (lr: PPB.leaf_reader (parse_bounded_integer (log256' max)))
+  (u: squash FStar.SizeT.fits_u64)
+: PPB.zero_copy_parse vmatch (parse_bounded_vldata min max p)
+= zero_copy_parse_bounded_vldata_payload' min max (log256' max) w lr u
